Complete proofs wp rules: Lea, Restrict, Seal, Unseal, AddSubLt, Store

theories/rules/rules_Restrict.v
@@ -70,141 +70,182 @@ Section cap_lang_rules.
       Restrict_failure lregs dst src →
       Restrict_spec lregs dst src lregs' FailedV.
 
-  Lemma wp_Restrict Ep pc_p pc_b pc_e pc_a pc_v pca_v lw dst src lregs :
+  Definition exec_optL_Restrict
+    (lregs : LReg) (dst: RegName) (src: Z + RegName) : option LReg :=
+    n ← z_of_argumentL lregs src;
+    lwdst ← lregs !! dst ;
+    match lwdst with
+    | LCap permPair b e a v =>
+        match permPair with
+        | E => None
+        | _ => if PermFlowsTo (decodePerm n) permPair
+              then
+                lregs' ← incrementLPC ( <[dst := (LCap (decodePerm n) b e a v) ]> lregs) ;
+                Some lregs'
+              else None
+        end
+    | LSealRange p b e a =>
+        if SealPermFlowsTo (decodeSealPerms n) p
+        then
+          lregs' ← incrementLPC ( <[dst := (LSealRange (decodeSealPerms n) b e a) ]> lregs) ;
+          Some lregs'
+        else None
+    | _ => None
+    end.
+
+  (* TODO move *)
+  Lemma rewrite_invert_match_E {R: Type} (X Y : R) (p : Perm) :
+    p ≠ E ->
+    (match p with
+     | E => Y
+     | _ => X
+     end) = X.
+  Proof.
+    intros.
+    destruct p ; cbn in *; done.
+  Qed.
+
+  Lemma wp_Restrict Ep pc_p pc_b pc_e pc_a pc_v lw dst src lregs :
     decodeInstrWL lw = Restrict dst src ->
     isCorrectLPC (LCap pc_p pc_b pc_e pc_a pc_v) →
     lregs !! PC = Some (LCap pc_p pc_b pc_e pc_a pc_v) →
     regs_of (Restrict dst src) ⊆ dom lregs →
 
-    {{{ ▷ (pc_a, pca_v) ↦ₐ lw ∗
+    {{{ ▷ (pc_a, pc_v) ↦ₐ lw ∗
         ▷ [∗ map] k↦y ∈ lregs, k ↦ᵣ y }}}
       Instr Executable @ Ep
     {{{ lregs' retv, RET retv;
         ⌜ Restrict_spec lregs dst src lregs' retv ⌝ ∗
-        (pc_a, pca_v) ↦ₐ lw ∗
+        (pc_a, pc_v) ↦ₐ lw ∗
         [∗ map] k↦y ∈ lregs', k ↦ᵣ y }}}.
   Proof.
-    (* iIntros (Hinstr Hvpc HPC Dregs φ) "(>Hpc_a & >Hmap) Hφ". *)
-    (* iApply wp_lift_atomic_head_step_no_fork; auto. *)
-    (* iIntros (σ1 ns l1 l2 nt) "Hσ1 /=". destruct σ1; simpl. *)
-    (* iDestruct "Hσ1" as "[Hr Hm]". *)
-    (* iDestruct (gen_heap_valid_inclSepM with "Hr Hmap") as %Hregs. *)
-    (* have ? := lookup_weaken _ _ _ _ HPC Hregs. *)
-    (* iDestruct (@gen_heap_valid with "Hm Hpc_a") as %Hpc_a; auto. *)
-    (* iModIntro. iSplitR. by iPureIntro; apply normal_always_head_reducible. *)
-    (* iNext. iIntros (e2 σ2 efs Hpstep). *)
-    (* apply prim_step_exec_inv in Hpstep as (-> & -> & (c & -> & Hstep)). *)
-    (* iIntros "_". *)
-    (* iSplitR; auto. eapply step_exec_inv in Hstep; eauto. *)
+    iIntros (Hinstr Hvpc HPC Dregs φ) "(>Hpc_a & >Hmap) Hφ".
+    cbn in Dregs.
+    iApply (wp_instr_exec_opt Hvpc HPC Hinstr Dregs with "[$Hpc_a $Hmap Hφ]").
+    iModIntro.
+    iIntros (σ1) "(Hσ1 & Hmap &Hpc_a)".
+    iModIntro.
+    iIntros (wa) "(%Hrpc & %Hmema & %Hcorrpc & %Hdecode) Hcred".
 
-    (* specialize (indom_regs_incl _ _ _ Dregs Hregs) as Hri. *)
-    (* unfold regs_of in Hri, Dregs. *)
-    (* destruct (Hri dst) as [wdst [H'dst Hdst]]. by set_solver+. *)
+    iApply (wp_wp2 (φ1 := exec_optL_Restrict lregs dst src)).
 
-    (* rewrite /exec /= Hdst /= in Hstep. *)
+    iMod (state_interp_transient_intro (lm:= ∅) with "[$Hmap $Hσ1]") as "Hσ".
+    { by rewrite big_sepM_empty. }
 
-    (* destruct (z_of_argument regs src) as [wsrc|] eqn:Hwsrc; *)
-    (*   pose proof Hwsrc as H'wsrc; cycle 1. *)
-    (*  { (* Failure: argument is not a constant (z_of_argument regs arg = None) *) *)
-    (*    unfold z_of_argument in Hwsrc, Hstep. destruct src as [| r0]; [ congruence |]. *)
-    (*    odestruct (Hri r0) as [r0v [Hr'0 Hr0]]. *)
-    (*    { unfold regs_of_argument. set_solver+. } *)
-    (*    rewrite Hr0 Hr'0 in Hwsrc Hstep. *)
-    (*    assert (c = Failed ∧ σ2 = {| reg := reg ; mem := mem ; etable := etable ; enumcur := enumcur |}) as (-> & ->). *)
-    (*    { destruct_word r0v; cbn in Hstep; try congruence; by simplify_pair_eq. } *)
-    (*    iFailWP "Hφ" Restrict_fail_src_nonz. } *)
-    (* apply (z_of_arg_mono _ reg) in Hwsrc; auto. rewrite Hwsrc in Hstep; simpl in Hstep. *)
+    iApply wp_opt2_bind.
+    iApply wp_opt2_eqn_both.
+    iApply (wp2_z_of_argument with "[Hφ Hpc_a Hcred $Hσ]"); first set_solver.
+    iSplit.
+    { iIntros "Hσ %Heqn1 %Heqn2".
+      iDestruct (state_interp_transient_elim_abort with "Hσ") as "($ & Hregs & _)".
+      iApply ("Hφ" with "[$Hpc_a $Hregs]").
+      iPureIntro.
+      eapply Restrict_spec_failure.
+      by constructor.
+    }
+    iIntros ( n_perm ) "Hσ %HsrcL %Hsrc".
 
-    (* destruct (is_mutable_range wdst) eqn:Hwdst. *)
-    (*  2: { (* Failure: wdst is not of the right type *) *)
-    (*    unfold is_mutable_range in Hwdst. *)
-    (*    assert (c = Failed ∧ σ2 = {| reg := reg ; mem := mem ; etable := etable ; enumcur := enumcur |}) as (-> & ->). *)
-    (*    { destruct wdst as [ | [p b e a | ] | ]; try by inversion Hwdst. *)
-    (*      all: try by simplify_pair_eq. *)
-    (*      destruct p; try congruence. *)
-    (*      simplify_pair_eq; auto. } *)
-    (*    iFailWP "Hφ" Restrict_fail_allowed. } *)
+    iApply wp_opt2_bind.
+    iApply wp_opt2_eqn_both.
+    iApply (wp2_reg_lookup with "[$Hσ Hφ Hcred Hpc_a]") ; first by set_solver.
+    iIntros (lwdst) "Hσ %HdstL %Hdst".
 
-    (* (* Now the proof splits depending on the type of value in wdst *) *)
-    (* destruct wdst as [ | [p b e a | p b e a] | ]. *)
-    (* 1,4: inversion Hwdst. *)
+    destruct (decide (is_mutable_rangeL lwdst = true)) as [HmutRange|HmutRange]
+    ; cycle 1.
+    (* case LInt or LSealed : fail *)
+    {
+      rewrite not_true_iff_false in HmutRange.
+      destruct_lword lwdst ; [ |  destruct p | | |] ; cbn in * ; simplify_eq.
+      all: iModIntro.
+      all: iDestruct (state_interp_transient_elim_abort with "Hσ") as "($ & Hregs & _)".
+      all: iApply ("Hφ" with "[$Hpc_a $Hregs]").
+      all: iPureIntro; econstructor; by eapply Restrict_fail_allowed.
+    }
 
-    (*  (* First, the case where r1v is a capability *) *)
-    (*  + destruct (perm_eq_dec p E); [ subst p |]. *)
-    (*    { rewrite /is_mutable_range in Hwdst; congruence. } *)
+    destruct_lword lwdst ; cbn in * ; simplify_eq.
+    - (* case LCap *)
+      destruct (decide (p = E)) as [HpE|HnpE]; subst; first done.
+      rewrite !rewrite_invert_match_E //=.
+      destruct (PermFlowsTo (decodePerm n_perm) p) eqn:Hflow ; cycle 1.
+      {
+        destruct p ; cbn in * ; simplify_eq.
+        all: iModIntro.
+        all: iDestruct (state_interp_transient_elim_abort with "Hσ") as "($ & Hregs & _)".
+        all: iApply ("Hφ" with "[$Hpc_a $Hregs]").
+        all: iPureIntro; econstructor; by eapply Restrict_fail_invalid_perm_cap.
+      }
 
-    (*    destruct (PermFlowsTo (decodePerm wsrc) p) eqn:Hflows; cycle 1. *)
-    (*    { destruct p; try congruence; inv Hstep ; iFailWP "Hφ" Restrict_fail_invalid_perm_cap. } *)
-    (*    rewrite /update_reg /= in Hstep. *)
+      iDestruct (update_state_interp_transient_from_regs_mod (dst := dst) (lw2 := LCap (decodePerm n_perm) b e a v) with "Hσ") as "Hσ".
+      { now set_solver. }
+      { intros.
+        eapply is_cur_lword_lea; eauto; eauto.
+      }
 
-    (*    destruct (incrementPC (<[ dst := WCap (decodePerm wsrc) b e a ]> regs)) eqn:Hregs'; *)
-    (*      pose proof Hregs' as H'regs'; cycle 1. *)
-    (*    { *)
-    (*      assert (incrementPC (<[ dst := WCap( decodePerm wsrc) b e a ]> reg) = None) as HH. *)
-    (*      { eapply incrementPC_overflow_mono; first eapply Hregs'. *)
-    (*          by rewrite lookup_insert_is_Some'; eauto. *)
-    (*            by apply insert_mono; eauto. } *)
-    (*      eapply (incrementPC_fail_updatePC _ mem) in HH. rewrite HH in Hstep. *)
-    (*      assert (c = Failed ∧ σ2 = {| reg := reg ; mem := mem ; etable := etable ; enumcur := enumcur |}) as (-> & ->) *)
-    (*          by (destruct p; inversion Hstep; auto). *)
-    (*      iFailWP "Hφ" Restrict_fail_PC_overflow_cap. } *)
+      rewrite updatePC_incrementPC.
+      iApply (wp_opt2_bind (k1 := fun x => Some x)).
+      iApply wp_opt2_eqn_both.
+      iApply (wp2_opt_incrementPC (φ := σ1) (lr := lregs) (lrt := <[ dst := LCap (decodePerm n_perm) b e a v]> lregs)).
+      { now rewrite elem_of_dom (lookup_insert_dec HPC). }
+      iFrame "Hσ".
+      iSplit; cbn.
+      + iIntros (φt' lrt') "Hσ %Hlin %Hin".
+        iDestruct (state_interp_transient_elim_abort with "Hσ") as "($ & Hregs & _)".
+        iApply ("Hφ" with "[$Hpc_a $Hregs]").
+        iPureIntro; constructor ; by eapply Restrict_fail_PC_overflow_cap.
+      + iIntros (lrt' rs') "Hσ %Hlis %His".
+        cbn.
+        iMod (state_interp_transient_elim_commit with "Hσ") as "($ & Hregs & _)".
+        iApply ("Hφ" with "[$Hpc_a $Hregs]").
+        iPureIntro.
+        by eapply Restrict_spec_success_cap.
 
-    (*    eapply (incrementPC_success_updatePC _ mem) in Hregs' *)
-    (*      as (p' & g' & b' & e' & a'' & a_pc' & HPC'' & HuPC & ->). *)
-    (*    eapply updatePC_success_incl with (m':=mem) in HuPC. 2: by eapply insert_mono; eauto. rewrite HuPC in Hstep. *)
-    (*    eassert ((c, σ2) = (NextI, _)) as HH. *)
-    (*    { destruct p; cbn in Hstep; eauto. congruence. } *)
-    (*    simplify_pair_eq. *)
+    - (* case LSealable *)
+      destruct (SealPermFlowsTo (decodeSealPerms n_perm) p) eqn:Hflow ; cycle 1.
+      {
+        destruct p ; cbn in * ; simplify_eq.
+        all: iModIntro.
+        all: iDestruct (state_interp_transient_elim_abort with "Hσ") as "($ & Hregs & _)".
+        all: iApply ("Hφ" with "[$Hpc_a $Hregs]").
+        all: iPureIntro; econstructor; by eapply Restrict_fail_invalid_perm_sr.
+      }
 
-    (*    iFrame. *)
-    (*    iMod ((gen_heap_update_inSepM _ _ dst) with "Hr Hmap") as "[Hr Hmap]"; eauto. *)
-    (*    iMod ((gen_heap_update_inSepM _ _ PC) with "Hr Hmap") as "[Hr Hmap]"; eauto. *)
-    (*    iFrame. iApply "Hφ". iFrame. iPureIntro. econstructor; eauto. *)
-    (*  (* Now, the case where wsrc is a sealrange *) *)
-    (*  + destruct (SealPermFlowsTo (decodeSealPerms wsrc) p) eqn:Hflows; cycle 1. *)
-    (*    { destruct p; try congruence; inv Hstep ; iFailWP "Hφ" Restrict_fail_invalid_perm_sr. } *)
-    (*    rewrite /update_reg /= in Hstep. *)
+      iDestruct (update_state_interp_transient_from_regs_mod (dst := dst)
+                   (lw2 := LSealRange (decodeSealPerms n_perm) b e a) with "Hσ") as "Hσ".
+      { now set_solver. }
+      { by intros; cbn. }
 
-    (*    destruct (incrementPC (<[ dst := WSealRange (decodeSealPerms wsrc) b e a ]> regs)) eqn:Hregs'; *)
-    (*      pose proof Hregs' as H'regs'; cycle 1. *)
-    (*    { *)
-    (*      assert (incrementPC (<[ dst := WSealRange (decodeSealPerms wsrc) b e a ]> reg) = None) as HH. *)
-    (*      { eapply incrementPC_overflow_mono; first eapply Hregs'. *)
-    (*          by rewrite lookup_insert_is_Some'; eauto. *)
-    (*            by apply insert_mono; eauto. } *)
-    (*      eapply (incrementPC_fail_updatePC _ mem) in HH. rewrite HH in Hstep. *)
-    (*      assert (c = Failed ∧ σ2 = {| reg := reg ; mem := mem ; etable := etable ; enumcur := enumcur |}) as (-> & ->) *)
-    (*          by (destruct p; inversion Hstep; auto). *)
-    (*      iFailWP "Hφ" Restrict_fail_PC_overflow_sr. } *)
+      rewrite updatePC_incrementPC.
+      iApply (wp_opt2_bind (k1 := fun x => Some x)).
+      iApply wp_opt2_eqn_both.
+      iApply (wp2_opt_incrementPC (φ := σ1) (lr := lregs) (lrt := <[ dst := LSealRange (decodeSealPerms n_perm) b e a]> lregs)).
+      { now rewrite elem_of_dom (lookup_insert_dec HPC). }
+      iFrame "Hσ".
+      iSplit; cbn.
+      + iIntros (φt' lrt') "Hσ %Hlin %Hin".
+        iDestruct (state_interp_transient_elim_abort with "Hσ") as "($ & Hregs & _)".
+        iApply ("Hφ" with "[$Hpc_a $Hregs]").
+        iPureIntro; constructor ; by eapply Restrict_fail_PC_overflow_sr.
+      + iIntros (lrt' rs') "Hσ %Hlis %His".
+        cbn.
+        iMod (state_interp_transient_elim_commit with "Hσ") as "($ & Hregs & _)".
+        iApply ("Hφ" with "[$Hpc_a $Hregs]").
+        iPureIntro.
+        by eapply Restrict_spec_success_sr.
+  Qed.
 
-    (*    eapply (incrementPC_success_updatePC _ mem) in Hregs' *)
-    (*      as (p' & g' & b' & e' & a'' & a_pc' & HPC'' & HuPC & ->). *)
-    (*    eapply updatePC_success_incl with (m':=mem) in HuPC. 2: by eapply insert_mono; eauto. rewrite HuPC in Hstep. *)
-    (*    eassert ((c, σ2) = (NextI, _)) as HH. *)
-    (*    { destruct p; cbn in Hstep; eauto. } *)
-    (*    simplify_pair_eq. *)
-
-    (*    iFrame. *)
-    (*    iMod ((gen_heap_update_inSepM _ _ dst) with "Hr Hmap") as "[Hr Hmap]"; eauto. *)
-    (*    iMod ((gen_heap_update_inSepM _ _ PC) with "Hr Hmap") as "[Hr Hmap]"; eauto. *)
-    (*    iFrame. iApply "Hφ". iFrame. iPureIntro. econstructor 2; eauto. *)
-    (*    Unshelve. all: auto. *)
-  (* Qed. *)
-  Admitted.
-
-  Lemma wp_restrict_success_reg_PC Ep pc_p pc_b pc_e pc_a pc_v pca_v pc_a' lw rv z:
+  Lemma wp_restrict_success_reg_PC Ep pc_p pc_b pc_e pc_a pc_v pc_a' lw rv z:
     decodeInstrWL lw = Restrict PC (inr rv) →
     isCorrectLPC (LCap pc_p pc_b pc_e pc_a pc_v) →
     (pc_a + 1)%a = Some pc_a' →
     PermFlowsTo (decodePerm z) pc_p = true →
 
      {{{ ▷ PC ↦ᵣ LCap pc_p pc_b pc_e pc_a pc_v
-         ∗ ▷ (pc_a, pca_v) ↦ₐ lw
+         ∗ ▷ (pc_a, pc_v) ↦ₐ lw
          ∗ ▷ rv ↦ᵣ LInt z }}}
        Instr Executable @ Ep
        {{{ RET NextIV;
            PC ↦ᵣ LCap (decodePerm z) pc_b pc_e pc_a' pc_v
-           ∗ (pc_a, pca_v) ↦ₐ lw
+           ∗ (pc_a, pc_v) ↦ₐ lw
            ∗ rv ↦ᵣ LInt z }}}.
    Proof.
      iIntros (Hinstr Hvpc Hpca' Hflows ϕ) "(>HPC & >Hpc_a & >Hrv) Hφ".
@@ -229,7 +270,7 @@ Section cap_lang_rules.
        incrementLPC_inv; simplify_map_eq; eauto. congruence. }
    Qed.
 
-   Lemma wp_restrict_success_reg Ep pc_p pc_b pc_e pc_a pc_v pca_v pc_a' w r1 rv p b e a v z :
+   Lemma wp_restrict_success_reg Ep pc_p pc_b pc_e pc_a pc_v pc_a' w r1 rv p b e a v z :
      decodeInstrWL w = Restrict r1 (inr rv) →
      isCorrectLPC (LCap pc_p pc_b pc_e pc_a pc_v) →
      (pc_a + 1)%a = Some pc_a' →
@@ -237,13 +278,13 @@ Section cap_lang_rules.
      p ≠ E →
 
      {{{ ▷ PC ↦ᵣ LCap pc_p pc_b pc_e pc_a pc_v
-         ∗ ▷ (pc_a, pca_v) ↦ₐ w
+         ∗ ▷ (pc_a, pc_v) ↦ₐ w
          ∗ ▷ r1 ↦ᵣ LCap p b e a v
          ∗ ▷ rv ↦ᵣ LInt z }}}
        Instr Executable @ Ep
        {{{ RET NextIV;
            PC ↦ᵣ LCap pc_p pc_b pc_e pc_a' pc_v
-           ∗ (pc_a, pca_v) ↦ₐ w
+           ∗ (pc_a, pc_v) ↦ₐ w
            ∗ rv ↦ᵣ LInt z
            ∗ r1 ↦ᵣ LCap (decodePerm z) b e a v }}}.
    Proof.
@@ -267,18 +308,18 @@ Section cap_lang_rules.
       incrementLPC_inv; simplify_map_eq; eauto. congruence. }
    Qed.
 
-   Lemma wp_restrict_success_z_PC Ep pc_p pc_b pc_e pc_a pc_v pca_v pc_a' lw z :
+   Lemma wp_restrict_success_z_PC Ep pc_p pc_b pc_e pc_a pc_v pc_a' lw z :
      decodeInstrWL lw = Restrict PC (inl z) →
      isCorrectLPC (LCap pc_p pc_b pc_e pc_a pc_v) →
      (pc_a + 1)%a = Some pc_a' →
      PermFlowsTo (decodePerm z) pc_p = true →
 
      {{{ ▷ PC ↦ᵣ LCap pc_p pc_b pc_e pc_a pc_v
-         ∗ ▷ (pc_a, pca_v) ↦ₐ lw }}}
+         ∗ ▷ (pc_a, pc_v) ↦ₐ lw }}}
        Instr Executable @ Ep
      {{{ RET NextIV;
          PC ↦ᵣ LCap (decodePerm z) pc_b pc_e pc_a' pc_v
-         ∗ (pc_a, pca_v) ↦ₐ lw }}}.
+         ∗ (pc_a, pc_v) ↦ₐ lw }}}.
    Proof.
      iIntros (Hinstr Hvpc Hpca' Hflows ϕ) "(>HPC & >Hpc_a) Hφ".
      iDestruct (map_of_regs_1 with "HPC") as "Hmap".
@@ -302,7 +343,7 @@ Section cap_lang_rules.
        incrementLPC_inv; simplify_map_eq; eauto. congruence. }
    Qed.
 
-   Lemma wp_restrict_success_z Ep pc_p pc_b pc_e pc_a pc_v pca_v pc_a' lw r1 p b e a v z :
+   Lemma wp_restrict_success_z Ep pc_p pc_b pc_e pc_a pc_v pc_a' lw r1 p b e a v z :
      decodeInstrWL lw = Restrict r1 (inl z) →
      isCorrectLPC (LCap pc_p pc_b pc_e pc_a pc_v) →
      (pc_a + 1)%a = Some pc_a' →
@@ -310,12 +351,12 @@ Section cap_lang_rules.
      p ≠ E →
 
      {{{ ▷ PC ↦ᵣ LCap pc_p pc_b pc_e pc_a pc_v
-         ∗ ▷ (pc_a, pca_v) ↦ₐ lw
+         ∗ ▷ (pc_a, pc_v) ↦ₐ lw
          ∗ ▷ r1 ↦ᵣ LCap p b e a v }}}
        Instr Executable @ Ep
      {{{ RET NextIV;
          PC ↦ᵣ LCap pc_p pc_b pc_e pc_a' pc_v
-         ∗ (pc_a, pca_v) ↦ₐ lw
+         ∗ (pc_a, pc_v) ↦ₐ lw
          ∗ r1 ↦ᵣ LCap (decodePerm z) b e a v }}}.
    Proof.
      iIntros (Hinstr Hvpc Hpca' Hflows HpE ϕ) "(>HPC & >Hpc_a & >Hr1) Hφ".
@@ -342,20 +383,20 @@ Section cap_lang_rules.
 
    (* Similar rules in case we have a SealRange instead of a capability, where some cases are impossible, because a SealRange is not a valid PC *)
 
- Lemma wp_restrict_success_reg_sr Ep pc_p pc_b pc_e pc_a pc_v pca_v pc_a' lw r1 rv p (b e a : OType) z :
+ Lemma wp_restrict_success_reg_sr Ep pc_p pc_b pc_e pc_a pc_v pc_a' lw r1 rv p (b e a : OType) z :
      decodeInstrWL lw = Restrict r1 (inr rv) →
      isCorrectLPC (LCap pc_p pc_b pc_e pc_a pc_v) →
      (pc_a + 1)%a = Some pc_a' →
      SealPermFlowsTo (decodeSealPerms z) p = true →
 
      {{{ ▷ PC ↦ᵣ LCap pc_p pc_b pc_e pc_a pc_v
-         ∗ ▷ (pc_a, pca_v) ↦ₐ lw
+         ∗ ▷ (pc_a, pc_v) ↦ₐ lw
          ∗ ▷ r1 ↦ᵣ LSealRange p b e a
          ∗ ▷ rv ↦ᵣ LInt z }}}
        Instr Executable @ Ep
        {{{ RET NextIV;
            PC ↦ᵣ LCap pc_p pc_b pc_e pc_a' pc_v
-           ∗ (pc_a, pca_v) ↦ₐ lw
+           ∗ (pc_a, pc_v) ↦ₐ lw
            ∗ rv ↦ᵣ LInt z
            ∗ r1 ↦ᵣ LSealRange (decodeSealPerms z) b e a }}}.
    Proof.
@@ -378,19 +419,19 @@ Section cap_lang_rules.
       incrementLPC_inv; simplify_map_eq; eauto. congruence. }
    Qed.
 
-   Lemma wp_restrict_success_z_sr Ep pc_p pc_b pc_e pc_a pc_v pca_v pc_a' lw r1 p (b e a : OType) z :
+   Lemma wp_restrict_success_z_sr Ep pc_p pc_b pc_e pc_a pc_v pc_a' lw r1 p (b e a : OType) z :
      decodeInstrWL lw = Restrict r1 (inl z) →
      isCorrectLPC (LCap pc_p pc_b pc_e pc_a pc_v) →
      (pc_a + 1)%a = Some pc_a' →
      SealPermFlowsTo (decodeSealPerms z) p = true →
 
      {{{ ▷ PC ↦ᵣ LCap pc_p pc_b pc_e pc_a pc_v
-         ∗ ▷ (pc_a, pca_v) ↦ₐ lw
+         ∗ ▷ (pc_a, pc_v) ↦ₐ lw
          ∗ ▷ r1 ↦ᵣ LSealRange p b e a }}}
        Instr Executable @ Ep
      {{{ RET NextIV;
            PC ↦ᵣ LCap pc_p pc_b pc_e pc_a' pc_v
-         ∗ (pc_a, pca_v) ↦ₐ lw
+         ∗ (pc_a, pc_v) ↦ₐ lw
          ∗ r1 ↦ᵣ LSealRange (decodeSealPerms z) b e a }}}.
    Proof.
      iIntros (Hinstr Hvpc Hpca' Hflows ϕ) "(>HPC & >Hpc_a & >Hr1) Hφ".
